\documentclass[../main.tex]{subfiles}

\begin{document}
\chapter{Implicit Differentiation and Inverses}
\section{Implicit Differentiation}
We know:
\[ \frac{d}{dx} x^a = ax^{a-1} \quad \mid \quad a \in \mathbb{Z} \]
We will now extend this formula to cover $\mathbb{Q}$ as well:
\[
    a = \frac{m}{n} \rightarrow y = x^{\frac{m}{n}}
    \quad \mid \quad
    m, n \in \mathbb{Z}
\]
We can start computing the derivative using the chain rule:
\begin{align*}
    y^n &= x^n\\
    \frac{d}{dx} \left( y^n \right) &= \frac{d}{dx} \left( x^m \right)\\
    \frac{d}{dy} \left( y^n \right) \cdot \frac{dy}{dx} &= mx^{m - 1}\\
    \frac{dy}{dx} \left( ny^{n - 1} \right) &= mx^{m - 1}\\
\end{align*}
We finally have an expression for $y'$:
\begin{align*}
    \frac{dy}{dx} &= \frac{mx^{m - 1}}{ny^{n - 1}}\\
    &= \frac{m}{n} \cdot \frac{x^{m - 1}}{y^{n - 1}}\\
    &= \frac{m}{n} \cdot \frac{x^{m - 1}}{\left( x^{\frac{m}{n}} \right)^{n - 1}}\\
    &= ax^{m - 1 - \frac{m}{n}(n - 1)}\\
    &= ax^{a - 1}\\
    \therefore \frac{d}{dx} x^a &= ax^{a - 1} \quad \mid \quad a \in \mathbb{Q}
\end{align*}
\begin{exmp}
    The equation of a unit circle is:
    \[ y^2 = 1 - x^2 \]
    This can be rewritten as:
    \[ y = \left( 1 - x^2 \right)^{\frac{1}{2}} \]
    We can compute the derivative using the chain rule:
    \begin{align*}
        \frac{dy}{dx} &= \frac{1}{2} \left( 1 - x^2 \right)^{\frac{1}{2} - 1} \cdot (-2x)\\
        &= \frac{-x}{\left( 1 - x^2 \right)^{\frac{1}{2}}}\\
        &= - \frac{x}{y}
    \end{align*}
    However, we can do the same thing using \emph{implicit differentiation}:
    \begin{align*}
        x^2 + y^2 &= 1\\
        \frac{d}{dx} \left( x^2 + y^2 \right) &= \frac{d}{dx} (1)\\
        \frac{d}{dx} \left( x^2 \right) + \frac{d}{dx} \left( y^2 \right) &= 0\\
        2x + \frac{d}{dy} \left( y^2 \right) \cdot \frac{dy}{dx} &= 0\\
        2x + 2y y' &= 0\\
        y' &= - \frac{x}{y}
    \end{align*}
\end{exmp}
\begin{exmp}
    In the following case, it is not so easy to solve for $y$:
    \[ y^3 +xy^2 + 1 = 0 \]
    We will need to use implicit differentiation to find the derivative:
    \begin{align*}
        3y^2y' + y^2 + 2xyy' + 0 &= 0\\
        y' \left( 3y^2 + 2xy \right) &= -y^2\\
        y' &= - \frac{y^2}{3y^2 + 2xy}
    \end{align*}
\end{exmp}
\section{Inverses}
If $y = f(x)$ and $g(y) = x$, we call $g$ the \emph{inverse} of $f$, 
denoted $f^{-1}$:
\[ x = g(y) = f^{-1}(y) \]
Now, we will use implicit differentiation to find the derivative 
of the inverse function:
\begin{align*}
    y &= f(x)\\
    f^{-1}(y) &= x\\
    \frac{d}{dx} \left( f^{-1}(y) \right) &= \frac{d}{dx}(x)\\
    \frac{d}{dy} \left( f^{-1}(y) \right) \cdot \frac{dy}{dx} &= 1\\
    \frac{d}{dy} \left( f^{-1}(y) \right) &= \frac{1}{\frac{dy}{dx}}\\
\end{align*}
\begin{exmp}
    The derivative of $y = \tan^{-1}(x)$:
    \begin{align*}
        \tan y &= x\\
        \frac{d}{dx} \left( \tan y \right) &= \frac{d}{dx}(x)\\
        \frac{d}{dy} \left( \tan y \right) \cdot \frac{dy}{dx} &= 1\\
        \left( \csc^2 y \right) \cdot \frac{dy}{dx} &= 1\\
        \frac{dy}{dx} &= \cos^2 y\\
        &= \cos^2 \left( \tan^{-1}(x) \right)
    \end{align*}
    This form is messy. We will use geometry to simplify:
\end{exmp}
\end{document}